replica.i.dfy
@@ -31,26 +31,6 @@ module Replica {
     && (forall x | x in prePreparesRcvd && prePreparesRcvd[x].Some? :: prePreparesRcvd[x].value.PrePrepare?)
   }
 
-  // TODO(hristo) move FullImap to a library. There's nothing Host-y about it.
-  predicate FullImap<K(!new),V>(im:imap<K,V>) {
-    forall k :: k in im
-  }
-
-  // Warning: Dafny automation black magic.
-  // Everything is in a FullImap! But sometimes Dafny seems unable
-  // to trigger that forall. (jonh suspects the issue is related to
-  // the map being a deeply-nested expression, since Dafny gets the
-  // proof no problem here where the map is a top-level object.)
-  // So this predicate does "nothing" logically (it's just 'true'),
-  // but has the 'ensures' side-effect of pointing out the 'in' expression
-  // we need.
-  predicate TriggerKeyInFullImap<K(!new),V>(k:K, m:imap<K,V>) 
-    requires FullImap(m)
-    ensures k in m
-  {
-    true
-  }
-
   // The Working Window data structure. Here Replicas keep the PrePrepare from the Primary
   // and the votes from all peers. Once a Client Operation is committed by a given Replica
   // to a specific Sequence ID (the Replica has collected the necessary quorum of votes from
